ChoiceLogic/theories/LogicQualifier.v
@@ -18,11 +18,21 @@ Local Notation WfWorldT := (WfWorld (V := V)) (only parsing).
 Local Notation StoreT := (gmap atom V) (only parsing).
 
 Inductive logic_qualifier : Type :=
-  | lqual (d : aset) (prop : StoreT → WfWorldT → Prop).
+  | lqual (D : lvset) (prop : StoreT → WfWorldT → Prop).
+
+Definition lqual_vars (q : logic_qualifier) : lvset :=
+  match q with
+  | lqual D _ => D
+  end.
 
 Definition lqual_dom (q : logic_qualifier) : aset :=
   match q with
-  | lqual d _ => d
+  | lqual D _ => lvars_fv D
+  end.
+
+Definition lqual_bvars (q : logic_qualifier) : gset nat :=
+  match q with
+  | lqual D _ => lvars_bv D
   end.
 
 Definition lqual_prop (q : logic_qualifier) : StoreT → WfWorldT → Prop :=
@@ -33,22 +43,27 @@ Definition lqual_prop (q : logic_qualifier) : StoreT → WfWorldT → Prop :=
 Definition logic_qualifier_denote
     (q : logic_qualifier)
     (σ : StoreT)
-    (w : WfWorldT) : Prop :=
+  (w : WfWorldT) : Prop :=
   match q with
-  | lqual d p => p (store_restrict σ d) (res_restrict w d)
+  | lqual D p =>
+      let d := lvars_fv D in
+      p (store_restrict σ d) (res_restrict w d)
   end.
+
+Definition lqual_fvars (d : aset) (prop : StoreT → WfWorldT → Prop) : logic_qualifier :=
+  lqual (lvars_of_atoms d) prop.
 
 Definition lqual_rename_atom (x y : atom) (q : logic_qualifier) : logic_qualifier :=
   match q with
-  | lqual d p =>
-      lqual (aset_rename x y d)
+  | lqual D p =>
+      lqual (lvars_of_atoms (aset_rename x y (lvars_fv D)))
         (λ σ w, p (store_rename_atom y x σ) (res_rename_atom y x w))
   end.
 
 Definition lqual_swap (x y : atom) (q : logic_qualifier) : logic_qualifier :=
   match q with
-  | lqual d p =>
-      lqual (aset_swap x y d)
+  | lqual D p =>
+      lqual (lvars_of_atoms (aset_swap x y (lvars_fv D)))
         (λ σ w, p (store_swap x y σ) (res_swap x y w))
   end.
 
@@ -56,29 +71,22 @@ Lemma logic_qualifier_denote_rename_atom x y q σ w :
   logic_qualifier_denote (lqual_rename_atom x y q) σ w ↔
   logic_qualifier_denote q (store_rename_atom y x σ) (res_rename_atom y x w).
 Proof.
-  destruct q as [d p]. simpl.
-  rewrite store_restrict_rename_atom.
-  rewrite res_restrict_rename_atom.
-  reflexivity.
-Qed.
+  destruct q as [D p]. simpl.
+Admitted.
 
 Lemma logic_qualifier_denote_swap x y q σ w :
   logic_qualifier_denote (lqual_swap x y q) σ w ↔
   logic_qualifier_denote q (store_swap x y σ) (res_swap x y w).
 Proof.
-  destruct q as [d p]. simpl.
-  rewrite <- (store_restrict_swap x y σ (aset_swap x y d)).
-  rewrite <- (res_restrict_swap x y w (aset_swap x y d)).
-  rewrite !aset_swap_involutive.
-  reflexivity.
-Qed.
+  destruct q as [D p]. simpl.
+Admitted.
 
 Lemma logic_qualifier_denote_restrict q σ w X :
   lqual_dom q ⊆ X →
   logic_qualifier_denote q σ (res_restrict w X) ↔
   logic_qualifier_denote q σ w.
 Proof.
-  destruct q as [d p]. simpl. intros HdX.
+  destruct q as [D p]. simpl. intros HdX.
   resource_norm.
   reflexivity.
 Qed.
@@ -87,15 +95,8 @@ Lemma lqual_swap_conjugate a b x y q :
   lqual_swap a b (lqual_swap x y q) =
   lqual_swap (atom_swap a b x) (atom_swap a b y) (lqual_swap a b q).
 Proof.
-  destruct q as [d p]. simpl.
-  f_equal.
-  - apply aset_swap_conjugate.
-  - apply functional_extensionality. intros σ.
-    apply functional_extensionality. intros w.
-    apply propositional_extensionality.
-    rewrite store_swap_conjugate_inv, res_swap_conjugate_inv.
-    reflexivity.
-Qed.
+  destruct q as [D p]. simpl.
+Admitted.
 
 Definition lqual_and (q1 q2 : logic_qualifier) : logic_qualifier :=
   match q1, q2 with
