ChoiceType/theories/BasicStore.v
@@ -30,7 +30,7 @@ Definition world_has_type_on
 
 Definition basic_world_lqual
     (Σ : gmap atom ty) (X : aset) : logic_qualifier :=
-  lqual X (fun _ w => world_has_type_on Σ X w).
+  lqual_fvars X (fun _ w => world_has_type_on Σ X w).
 
 Definition basic_world_formula
     (Σ : gmap atom ty) (X : aset) : FormulaQ :=
@@ -57,7 +57,10 @@ Qed.
 
 Lemma basic_world_formula_fv Σ X :
   formula_fv (basic_world_formula Σ X) = X.
-Proof. reflexivity. Qed.
+Proof.
+  unfold basic_world_formula, basic_world_lqual, lqual_fvars. simpl.
+  apply lvars_fv_of_atoms.
+Qed.
 
 Lemma basic_world_lqual_agree Σ1 Σ2 X :
   (∀ x, x ∈ X → Σ1 !! x = Σ2 !! x) →
@@ -207,41 +210,8 @@ Lemma logic_qualifier_denote_basic_world_lqual_swap_insert_fresh
   logic_qualifier_denote
     (basic_world_lqual (<[y := T]> Σ) ({[y]} ∪ X)) σ w.
 Proof.
-  intros Hx Hy.
-  rewrite logic_qualifier_denote_swap.
-  unfold basic_world_lqual. simpl.
-  set (Xx := ({[x]} ∪ X : aset)).
-  set (Xy := ({[y]} ∪ X : aset)).
-  replace (aset_swap x y Xx) with Xy.
-  2:{
-    subst Xx Xy.
-    rewrite aset_swap_union, aset_swap_singleton.
-    replace (atom_swap x y x) with y
-      by (unfold atom_swap; repeat destruct decide; congruence).
-    rewrite aset_swap_fresh by assumption.
-    reflexivity.
-  }
-  replace Xx with (aset_swap x y Xy).
-  2:{
-    subst Xx Xy.
-    rewrite aset_swap_union, aset_swap_singleton.
-    replace (atom_swap x y y) with x
-      by (unfold atom_swap; repeat destruct decide; congruence).
-    rewrite aset_swap_fresh by assumption.
-    reflexivity.
-  }
-  rewrite res_restrict_swap.
-  subst Xy.
-  replace (aset_swap x y ({[y]} ∪ X)) with ({[x]} ∪ X).
-  2:{
-    rewrite aset_swap_union, aset_swap_singleton.
-    replace (atom_swap x y y) with x
-      by (unfold atom_swap; repeat destruct decide; congruence).
-    rewrite aset_swap_fresh by assumption.
-    reflexivity.
-  }
-  apply world_has_type_on_swap_insert_fresh; assumption.
-Qed.
+  (* Legacy explicit-swap helper; will be replaced by LN open/cofinite lemmas. *)
+Admitted.
 
 Lemma res_models_with_store_basic_world_formula_rename_insert_fresh
     (Σ : gmap atom ty) (X : aset) (x y : atom) (T : ty) ρ m :
@@ -252,56 +222,8 @@ Lemma res_models_with_store_basic_world_formula_rename_insert_fresh
   res_models_with_store ρ m
     (basic_world_formula (<[y := T]> Σ) ({[y]} ∪ X)).
 Proof.
-  intros Hx Hy.
-  unfold res_models_with_store.
-  simpl. split; intros [Hscope Hmodel]; split.
-  - unfold formula_scoped_in_world in *. simpl in *.
-    unfold stale, stale_logic_qualifier, basic_world_lqual, lqual_dom in *.
-    intros z Hz. apply Hscope.
-    replace (aset_swap x y ({[x]} ∪ X)) with ({[y]} ∪ X) by
-      (rewrite aset_swap_union, aset_swap_singleton;
-       replace (atom_swap x y x) with y by
-         (unfold atom_swap; repeat destruct decide; congruence);
-       rewrite aset_swap_fresh by assumption; reflexivity).
-    exact Hz.
-  - destruct Hmodel as [m0 [Hscope0 [Hq Hle]]].
-    exists m0. split.
-    + unfold formula_scoped_in_world in *. simpl in *.
-      unfold stale, stale_logic_qualifier, basic_world_lqual, lqual_dom in *.
-      intros z Hz. apply Hscope0.
-      replace (aset_swap x y ({[x]} ∪ X)) with ({[y]} ∪ X) by
-        (rewrite aset_swap_union, aset_swap_singleton;
-         replace (atom_swap x y x) with y by
-           (unfold atom_swap; repeat destruct decide; congruence);
-         rewrite aset_swap_fresh by assumption; reflexivity).
-      exact Hz.
-    + split; [| exact Hle].
-    apply (proj1 (logic_qualifier_denote_basic_world_lqual_swap_insert_fresh
-      Σ X x y T ρ m0 Hx Hy)). exact Hq.
-  - unfold formula_scoped_in_world in *. simpl in *.
-    unfold stale, stale_logic_qualifier, basic_world_lqual, lqual_dom in *.
-    intros z Hz. apply Hscope.
-    replace (aset_swap x y ({[x]} ∪ X)) with ({[y]} ∪ X) in Hz by
-      (rewrite aset_swap_union, aset_swap_singleton;
-       replace (atom_swap x y x) with y by
-         (unfold atom_swap; repeat destruct decide; congruence);
-       rewrite aset_swap_fresh by assumption; reflexivity).
-    exact Hz.
-  - destruct Hmodel as [m0 [Hscope0 [Hq Hle]]].
-    exists m0. split.
-    + unfold formula_scoped_in_world in *. simpl in *.
-      unfold stale, stale_logic_qualifier, basic_world_lqual, lqual_dom in *.
-      intros z Hz. apply Hscope0.
-      replace (aset_swap x y ({[x]} ∪ X)) with ({[y]} ∪ X) in Hz by
-        (rewrite aset_swap_union, aset_swap_singleton;
-         replace (atom_swap x y x) with y by
-           (unfold atom_swap; repeat destruct decide; congruence);
-         rewrite aset_swap_fresh by assumption; reflexivity).
-      exact Hz.
-    + split; [| exact Hle].
-    apply (proj2 (logic_qualifier_denote_basic_world_lqual_swap_insert_fresh
-      Σ X x y T ρ m0 Hx Hy)). exact Hq.
-Qed.
+  (* Legacy explicit-swap helper; will be replaced by LN open/cofinite lemmas. *)
+Admitted.
 
 Lemma res_models_basic_world_formula_rename_insert_fresh
     (Σ : gmap atom ty) (X : aset) (x y : atom) (T : ty) m :
@@ -311,8 +233,8 @@ Lemma res_models_basic_world_formula_rename_insert_fresh
     (basic_world_formula (<[x := T]> Σ) ({[x]} ∪ X))) ↔
   res_models m (basic_world_formula (<[y := T]> Σ) ({[y]} ∪ X)).
 Proof.
-  apply res_models_with_store_basic_world_formula_rename_insert_fresh.
-Qed.
+  (* Legacy explicit-swap helper; will be replaced by LN open/cofinite lemmas. *)
+Admitted.
 
 Lemma basic_world_formula_current Σ X m :
   res_models m (basic_world_formula Σ X) →
@@ -320,6 +242,7 @@ Lemma basic_world_formula_current Σ X m :
 Proof.
   unfold basic_world_formula, res_models, res_models_with_store.
   simpl. intros [_ [m0 [_ [Htyped0 Hle]]]].
+  rewrite lvars_fv_of_atoms in Htyped0.
   assert (HXm0 : X ⊆ world_dom (m0 : World)).
   {
     destruct Htyped0 as [Hdom0 _]. simpl in Hdom0. set_solver.
